CoherenceTop.v

CoherenceTop.v
@@ -52,14 +52,113 @@ Inductive sub : typ -> typ -> Prop :=
   | SOr3 : forall t t1 t2, sub t t2 -> Atomic t ->
      sub t (OrT t1 t2).
 
+Lemma sand2_atomic : forall t1 t2 t3, sub t1 t3 -> Atomic t3 -> sub (AndT t1 t2) t3.
+Proof.
+intros.
+eapply SAnd2 in H; eauto.
+Qed.
 
-Hint Resolve STop SInt SFun SAnd1 SAnd2 SAnd3 SOr1 SOr2 SOr3.
+Lemma sand3_atomic : forall t1 t2 t3, sub t2 t3 -> Atomic t3 -> sub (AndT t1 t2) t3.
+Proof.
+intros.
+eapply SAnd3 in H; eauto.
+Qed.
+
+Lemma sor2_atomic : forall t1 t2 t3, sub t1 t2 -> Atomic t1 -> sub t1 (OrT t2 t3).
+Proof.
+intros.
+eapply SOr2 in H; eauto.
+Qed.
+
+Lemma sor3_atomic : forall t1 t2 t3, sub t1 t3 -> Atomic t1 -> sub t1 (OrT t2 t3).
+Proof.
+intros.
+eapply SOr3 in H; eauto.
+Qed.
+
+Hint Resolve STop SInt SFun SAnd1 SAnd2 SAnd3 SOr1 SOr2 SOr3
+             sand2_atomic sand3_atomic sor2_atomic sor3_atomic.
+
+Lemma inv_ands1 : forall t t1 t2, sub t (AndT t1 t2) -> sub t t1 /\ sub t t2.
+Proof.
+  intro t; induction t; intros.
+  - inversion H. auto.
+  - inversion H. auto.
+  - inversion H. auto.
+(* Case AndT *)
+  - inversion H. auto.
+    assert (sub t1 t0 /\ sub t1 t3).
+    auto.
+    split.
+    destruct H5; apply SAnd2; auto; inversion H4.
+    destruct H5; apply SAnd3; auto; inversion H4.
+    assert (sub t2 t0 /\ sub t2 t3).
+    auto.
+    split.
+    destruct H5; apply SAnd2; auto; inversion H4.
+    destruct H5; apply SAnd3; auto; inversion H4.
+(* Case OrT *)
+  - inversion H. auto.
+    assert (sub t1 t0 /\ sub t1 t3).
+    auto.
+    assert (sub t2 t0 /\ sub t2 t3).
+    auto.
+    split.
+    apply SOr1.
+    destruct H5. auto.
+    destruct H6. auto.
+    apply SOr1.
+    destruct H5. auto.
+    destruct H6. auto.
+Qed.
+
+Lemma inv_ors1 : forall t t2 t3, sub (OrT t2 t3) t -> sub t2 t /\ sub t3 t.
+Proof.
+  intro t; induction t; intros.
+  - inversion H; auto.
+  - inversion H; auto.
+  - inversion H; auto.
+(* Case AndT *)
+  - inversion H; auto.
+    assert (sub t0 t1 /\ sub t3 t1).
+    auto.
+    assert (sub t0 t2 /\ sub t3 t2).
+    auto.
+    split.
+    apply SAnd1.
+    destruct H5. auto.
+    destruct H6. auto.
+    apply SAnd1.
+    destruct H5. auto.
+    destruct H6. auto.
+(* Case OrT *)
+  - inversion H; auto.
+    assert (sub t0 t1 /\ sub t3 t1).
+    auto.
+    split.
+    apply SOr2.
+    destruct H5. auto.
+    inversion H4.
+    apply SOr2.
+    destruct H5. auto.
+    inversion H4.
+    assert (sub t0 t2 /\ sub t3 t2).
+    auto.
+    split.
+    apply SOr3.
+    destruct H5. auto.
+    inversion H4.
+    apply SOr3.
+    destruct H5. auto.
+    inversion H4.
+Qed.
 
 Lemma sub_refl: forall A, sub A A.
 Proof.
   intros.
   induction A; eauto.
-  apply SAnd1. apply SAnd2; eauto. admit.
+  apply SAnd1.
+  apply SAnd2; eauto. admit.
   apply SAnd3; eauto. admit.
   apply SOr1. apply SOr2; auto. admit.
   apply SOr3; eauto. admit.
@@ -70,16 +169,36 @@ Hint Resolve sub_refl.
 Inductive TopLike : typ -> Prop :=
   | TLTop  : TopLike TopT
   | TLAnd  : forall A B, TopLike A -> TopLike B -> TopLike (AndT A B)
-  | TLFun  : forall A B, TopLike B -> TopLike (FunT A B).
+  | TLOr1  : forall A B, TopLike A -> TopLike (OrT A B)
+  | TLOr2  : forall A B, TopLike B -> TopLike (OrT A B).
 
 
-Hint Resolve TLTop TLAnd TLFun.
+Hint Resolve TLTop TLAnd TLOr1 TLOr2.
 
 
 (* Disjointness: Specification *)
 
 Definition OrthoS (A B: typ) := forall C, sub A C -> sub B C -> 
                                   sub (AndT A B) C -> TopLike C.
+
+Definition TopLikeS (A: typ) := sub TopT A.
+
+Lemma completeTopLike : forall A, TopLikeS A -> TopLike A.
+Proof.
+intros.
+unfold TopLikeS in H.
+dependent induction H; eauto.
+Defined.
+
+Lemma soundTopLike : forall A, TopLike A -> TopLikeS A.
+Proof.
+intros.
+dependent induction H; eauto.
+ - unfold TopLikeS; auto.
+ - unfold TopLikeS; auto.
+ - unfold TopLikeS; auto.
+ - unfold TopLikeS; auto.
+Defined.
 
 (* Disjointness: Implementation *)
 
@@ -95,12 +214,26 @@ Inductive Ortho : typ -> typ -> Prop :=
   | OFunTInt : forall t1 t2, Ortho (FunT t1 t2) IntT
   | OFun1   : forall t1 t2 t3 t4, Ortho t2 t4 -> Ortho (FunT t1 t2) (FunT t3 t4)
 (*  | OFun2  : forall t1 t2 t3 t4, Ortho t1 t3 -> Ortho (FunT t1 t2) (FunT t3 t4) *)
-  | Or1 : forall t1 t2 t3, Ortho (OrT t1 t2) t3 -> Ortho t1 t3
-  | Or2 : forall t1 t2 t3, Ortho (OrT t1 t2) t3 -> Ortho t2 t3
-  | Or3 : forall t1 t2 t3, Ortho t1 (OrT t2 t3) -> Ortho t1 t2
-  | Or4 : forall t1 t2 t3, Ortho t1 (OrT t2 t3) -> Ortho t1 t3.
+  | Or1 : forall t1 t2 t3, Ortho t1 t2 -> Ortho t1 (OrT t2 t3)
+  | Or2 : forall t1 t2 t3, Ortho t1 t3 -> Ortho t1 (OrT t2 t3)
+  | Or3 : forall t1 t2 t3, Ortho t1 t3 -> Ortho (OrT t1 t2) t3
+  | Or4 : forall t1 t2 t3, Ortho t2 t3 -> Ortho (OrT t1 t2) t3.
 
-Hint Resolve OTop1 OTop2 OAnd1 OAnd2 OIntFunT OFunTInt OFun1 Or1 Or2 Or3 Or4.
+Hint Resolve OTop1 OTop2 OAnd1 OAnd2 OIntFunT OFunTInt Or1 OFun1 Or2 Or3 Or4.
+
+Lemma applyOrthoS : forall A B, OrthoS A B -> forall C, sub A C -> sub B C ->
+                      sub (AndT A B) C -> TopLike C.
+Proof.
+intros. destruct H with (C:=C); auto.
+Defined.
+
+Lemma applyOrtho : forall A B, Ortho A B -> forall C, sub A C -> sub B C -> 
+                    sub (AndT A B) C -> TopLike C.
+Proof.
+intros.
+dependent induction C; eauto.
+Admitted.
+
 
 (* Well-formed types *)
 
@@ -115,31 +248,95 @@ Lemma sym_orthos : forall t1 t2, OrthoS t1 t2 -> OrthoS t2 t1.
 Proof.
 intros.
 unfold OrthoS in *; intros.
-apply H; auto.
-apply SAnd2. auto.
-Admitted.
+dependent induction C; eauto.
+(* Case And *)
+- apply TLAnd.
+  apply IHC1.
+  apply inv_ands1 in H0; destruct H0; auto.
+  apply inv_ands1 in H1; destruct H1; auto.
+  apply inv_ands1 in H2; destruct H2; eauto.
+  apply IHC2.
+  apply inv_ands1 in H0; destruct H0; auto.
+  apply inv_ands1 in H1; destruct H1; auto.
+  apply inv_ands1 in H2; destruct H2; eauto.
+(* Case Or *)
+- dependent destruction H2; inversion H3.
+Defined.
 
 Lemma sym_ortho : forall t1 t2, Ortho t1 t2 -> Ortho t2 t1.
 Proof.
 intros.
-dependent induction H; eauto.
+- dependent induction H; eauto.
 Qed.
 
 Lemma inv_orthos_and: forall t1 t2 t3, OrthoS t1 (AndT t2 t3) -> OrthoS t1 t2 /\ OrthoS t1 t3.
 Proof.
+intros.
+split.
+ - unfold OrthoS; intros.
+   dependent induction C; eauto.
+  + apply TLAnd.
+    apply IHC1.
+    apply inv_ands1 in H0; destruct H0; auto.
+    apply inv_ands1 in H1; destruct H1; auto.
+    apply inv_ands1 in H2; destruct H2; auto.
+    apply IHC2.
+    apply inv_ands1 in H0; destruct H0; auto.
+    apply inv_ands1 in H1; destruct H1; auto.
+    apply inv_ands1 in H2; destruct H2; auto.
+  + dependent destruction H2; inversion H3.
+ - unfold OrthoS; intros.
+   dependent induction C; eauto.
+  + apply TLAnd.
+    apply IHC1.
+    apply inv_ands1 in H0; destruct H0; auto.
+    apply inv_ands1 in H1; destruct H1; auto.
+    apply inv_ands1 in H2; destruct H2; auto.
+    apply IHC2.
+    apply inv_ands1 in H0; destruct H0; auto.
+    apply inv_ands1 in H1; destruct H1; auto.
+    apply inv_ands1 in H2; destruct H2; auto.
+  + dependent destruction H2; inversion H3.
+Defined.
+
+Lemma inv_orthos_or : forall t1 t2, OrthoS t1 (OrT t1 t2) -> OrthoS t1 t2.
+Proof.
+intros.
+unfold OrthoS in H.
+unfold OrthoS. intros.
+dependent induction C; eauto.
+ - apply TLAnd.
+   apply IHC1.
+   apply inv_ands1 in H0; destruct H0; auto.
+   apply inv_ands1 in H1; destruct H1; auto.
+   apply inv_ands1 in H2; destruct H2; auto.
+   apply IHC2.
+   apply inv_ands1 in H0; destruct H0; auto.
+   apply inv_ands1 in H1; destruct H1; auto.
+   apply inv_ands1 in H2; destruct H2; auto.
+ - dependent destruction H2; inversion H3.
+Defined.
+
+Lemma inv_orthos_or2 : forall t1 t2 t3, OrthoS t1 (OrT t2 t3) -> OrthoS t1 t2 \/ OrthoS t1 t3.
+Proof.
+intros.
+left.
+unfold OrthoS; intros.
+unfold OrthoS in H.
+dependent induction C; auto.
+inversion H2.
+apply H; auto.
+apply SOr1; auto. admit.
+apply H; auto.
+apply SOr1; auto. admit.
 Admitted.
 
-Lemma inv_ortho_or : forall t1 t2 t3, Ortho t1 t2 -> Ortho t1 t3 -> Ortho t1 (OrT t2 t3).
+Lemma ortho_fun : forall t1 t2 t3 t4, Ortho (FunT t1 t2) (FunT t3 t4) 
+                          -> Ortho t2 t4. 
 Proof.
-Admitted.
-
-Lemma inv_orthos_or : forall t1 t2 t3, OrthoS t1 (OrT t2 t3) -> OrthoS t1 t2 /\ OrthoS t1 t3.
-Proof.
-Admitted.
-
-Lemma inv_orthos_fun : forall t1 t2 t3 t4, OrthoS (FunT t1 t2) (FunT t3 t4) -> OrthoS t2 t4.
-Proof.
-Admitted.
+intros.
+inversion H. auto.
+Defined.
 
 (* Soundness lemma of the disjointness algorithm *)
 
@@ -149,27 +346,32 @@ intros t1 wft1.
 induction wft1; intros.
 apply OTop2.
 (* Case IntT *)
-generalize H0. clear H0. induction H; intros; eauto.
+induction H; intros; eauto.
 unfold OrthoS in H0; eauto.
 assert (t0: TopLike IntT); auto. inversion t0.
 apply OAnd2. apply IHWFTyp1.
-apply inv_orthos_and in H2.
-destruct H2; auto. 
-apply inv_orthos_and in H2.
-destruct H2; auto.
-apply inv_ortho_or.
-apply IHWFTyp1.
-apply inv_orthos_or in H1.
-destruct H1; auto.
-apply IHWFTyp2.
-apply inv_orthos_or in H1.
-destruct H1; auto.
+apply inv_orthos_and in H0.
+destruct H0; auto. 
+apply inv_orthos_and in H0.
+destruct H0; auto.
+apply inv_orthos_or2 in H0.
+destruct H0.
+apply Or1.
+apply IHWFTyp1. auto.
+apply Or2.
+apply IHWFTyp2. auto.
 (* Case FunT t1 t2 *)
 induction H; eauto.
 (* Case FunT t1 t2 | FunT t0 t3 *)
 apply OFun1.
 apply IHwft1_2; eauto.
-apply inv_orthos_fun in H0. auto.
+unfold OrthoS in H0.
+unfold OrthoS. intros.
+assert (TopLike (FunT (AndT t1 t0) C)).
+apply H0.
+apply SFun. apply SAnd2. auto. admit. auto.
+apply SFun. apply SAnd3. auto. admit. auto.
+admit. admit.
 (* Case t11 -> t12 _|_ t21 & t22 *)
 apply OAnd2. apply IHWFTyp1.
 apply inv_orthos_and in H0.
@@ -178,13 +380,12 @@ apply IHWFTyp2.
 apply inv_orthos_and in H0.
 destruct H0; auto.
 (* Case t11 -> t12 _|_ t21 | t22 *)
-apply inv_ortho_or.
-apply IHWFTyp1.
-apply inv_orthos_or in H0.
-destruct H0; auto.
-apply IHWFTyp2.
-apply inv_orthos_or in H0.
-destruct H0; auto.
+apply inv_orthos_or2 in H0.
+destruct H0.
+apply Or1.
+apply IHWFTyp1. auto.
+apply Or2.
+apply IHWFTyp2. auto.
 (* Case (t11 & t12) _|_ t2 *)
 apply OAnd1.
 apply IHwft1_1; auto.
@@ -198,91 +399,145 @@ apply inv_orthos_and in H1.
 apply sym_orthos.
 destruct H1; auto.
 (* Case (t11 | t12) _|_ t2 *)
-apply sym_ortho.
-apply inv_ortho_or.
-apply sym_ortho.
-apply IHwft1_1; auto.
 apply sym_orthos in H0.
-apply inv_orthos_or in H0.
+apply inv_orthos_or2 in H0.
 destruct H0.
-apply sym_orthos; auto.
-apply sym_ortho.
-apply IHwft1_2; auto.
-apply sym_orthos in H0.
-apply inv_orthos_or in H0.
-destruct H0.
-apply sym_orthos; auto.
-Qed.
+apply Or3.
+apply IHwft1_1. auto.
+apply sym_orthos. auto.
+apply Or4.
+apply IHwft1_2. auto.
+apply sym_orthos. auto.
+Admitted.
 
 (* Soundness of the disjointness algorithm: Theorem 7 *)
 
+Lemma ortho_and : forall {A B C}, OrthoS A C -> OrthoS B C -> OrthoS (AndT A B) C.
+Proof.
+intros.
+unfold OrthoS. intros.
+unfold OrthoS in H.
+unfold OrthoS in H0.
+dependent induction C0; eauto.
+inversion H1.
+apply H; auto.
+apply H0; auto.
+inversion H1.
+apply H; auto.
+apply H0; auto.
+apply TLAnd.
+apply IHC0_1.
+apply inv_ands1 in H1. destruct H1. auto.
+apply inv_ands1 in H2. destruct H2. auto.
+apply inv_ands1 in H3. destruct H3. auto.
+apply IHC0_2.
+apply inv_ands1 in H1. destruct H1. auto.
+apply inv_ands1 in H2. destruct H2. auto.
+apply inv_ands1 in H3. destruct H3. auto.
+dependent destruction H3; inversion H4.
+Defined.
+
+Lemma orthos_or1 : forall {A B C}, OrthoS A C -> OrthoS (OrT A B) C.
+Proof.
+intros.
+unfold OrthoS in *.
+intros.
+apply H.
+apply inv_ors1 in H0. destruct H0. auto. auto.
+apply inv_ors1 in H0. destruct H0.
+eapply SAnd2 in H0; eauto.
+Admitted.
+
+Lemma orthos_or2 : forall {A B C}, OrthoS B C -> OrthoS (OrT A B) C.
+Proof.
+intros.
+unfold OrthoS in *.
+intros.
+apply H; eauto.
+apply inv_ors1 in H0. destruct H0. auto.
+apply inv_ors1 in H0. destruct H0.
+eapply SAnd2; eauto.
+Admitted.
+
 Lemma ortho_soundness : forall (t1 t2 : typ), WFTyp t1 -> WFTyp t2 -> Ortho t1 t2 -> OrthoS t1 t2.
 intros.
-induction H.
+induction H1.
 (*Case t1 TopT*)
-unfold OrthoS. intros.
-induction C; eauto. inversion H.
-apply TLFun. apply IHC2; auto.
-apply TLAnd. apply IHC1
-apply invAndS1 in H. destruct H. auto.
-apply invAndS1 in H0. destruct H0. auto.
+unfold OrthoS; intros.
+induction C; eauto. inversion H2. inversion H2.
+apply TLAnd. apply IHC1.
+apply inv_ands1 in H1. destruct H1. auto.
+apply inv_ands1 in H2. destruct H2. auto.
+apply inv_ands1 in H3. destruct H3. auto.
 apply IHC2.
-apply invAndS1 in H. destruct H. auto.
-apply invAndS1 in H0. destruct H0. auto.
-apply TLTop.
+apply inv_ands1 in H1. destruct H1. auto.
+apply inv_ands1 in H2. destruct H2. auto.
+apply inv_ands1 in H3. destruct H3. auto.
+dependent destruction H3; inversion H4.
 (*Case TopT t1*)
 unfold OrthoS. intros.
-induction C. inversion H. inversion H.
-apply TLAnd. apply IHC1.
-apply invAndS1 in H. destruct H. auto.
-apply invAndS1 in H0. destruct H0. auto.
-apply IHC2.
-apply invAndS1 in H. destruct H. auto.
-apply invAndS1 in H0. destruct H0. auto.
+induction C.
 apply TLTop.
-(* Hard case *)
-apply ortho_and; auto.
-assert (OrthoS t2 t1). apply ortho_sym. apply IHOrtho1; auto.
-assert (OrthoS t3 t1). apply ortho_sym. apply IHOrtho2; auto.
-apply ortho_sym.
-apply ortho_and; auto.
+inversion H1. inversion H1.
+apply TLAnd. apply IHC1.
+apply inv_ands1 in H1. destruct H1. auto.
+apply inv_ands1 in H2. destruct H2. auto.
+apply inv_ands1 in H3. destruct H3. auto.
+apply IHC2.
+apply inv_ands1 in H1. destruct H1. auto.
+apply inv_ands1 in H2. destruct H2. auto.
+apply inv_ands1 in H3. destruct H3. auto.
+dependent destruction H3; inversion H4.
+(* Hard case: (AndT t1 t2) t3 *)
+apply ortho_and.
+apply IHOrtho1; eauto. inversion H. auto.
+apply IHOrtho2; eauto. inversion H. auto.
+apply sym_orthos.
+apply ortho_and.
+apply sym_orthos.
+apply IHOrtho1; eauto. inversion H0. auto.
+apply sym_orthos.
+apply IHOrtho2; eauto. inversion H0. auto.
 (* Case IntFunT *)
 unfold OrthoS.
-induction C; intros. inversion H0. inversion H.
-apply TLAnd. apply IHC1. inversion H. auto. inversion H0. auto.
-apply IHC2. inversion H. auto. inversion H0. auto.
-(* TopT *)
-apply TLTop.
+induction C; intros. apply TLTop. inversion H2. inversion H1.
+apply TLAnd. apply IHC1. inversion H1. auto. inversion H2. auto.
+apply inv_ands1 in H3. destruct H3. auto.
+apply IHC2. inversion H1. auto. inversion H2. auto.
+apply inv_ands1 in H3. destruct H3. auto.
+dependent destruction H3; inversion H4.
 (* Case FunTInt *)
 unfold OrthoS.
-induction C; intros. inversion H. inversion H0.
+induction C; intros. apply TLTop. inversion H1. inversion H2.
 apply TLAnd.
-apply IHC1.
-inversion H. auto.
-inversion H0. auto.
-apply IHC2.
-inversion H. auto.
-inversion H0. auto.
-(* TopT *)
-apply TLTop.
+apply IHC1. inversion H1. auto. inversion H2. auto.
+apply inv_ands1 in H3. destruct H3. auto.
+apply IHC2. inversion H1. auto. inversion H2. auto.
+apply inv_ands1 in H3. destruct H3. auto.
+dependent destruction H3; inversion H4.
 (* FunTFunT *)
 unfold OrthoS.
 intros.
-induction C. inversion H0.
+induction C. apply TLTop. inversion H2.
 assert (Ortho (FunT t1 t2) (FunT t3 t4)).
-apply OFunT. auto.
-apply applyOrtho. auto. auto. auto.
-apply TLAnd. apply IHC1. inversion H0. auto. inversion H1. auto.
-apply IHC2. inversion H0. auto. inversion H1. auto.
-apply TLTop.
-(* FunTFunTA *)
-unfold OrthoS.
-intros.
-induction C. inversion H0.
-assert (Ortho (FunT t1 t2) (FunT t3 t4)).
-apply OFunTA. auto.
-apply applyOrtho. auto. auto. auto. auto.
-apply TLAnd. apply IHC1. inversion H0. auto. inversion H1. auto.
-apply IHC2. inversion H0. auto. inversion H1. auto.
-apply TLTop.
+apply OFun1. auto.
+eapply applyOrtho with (A:=(FunT t1 t2)) (B:=(FunT t3 t4)); eauto.
+apply TLAnd. apply IHC1. inversion H2. auto. inversion H3. auto.
+apply inv_ands1 in H4. destruct H4. auto.
+apply IHC2. inversion H2. auto. inversion H3. auto.
+apply inv_ands1 in H4. destruct H4. auto.
+dependent destruction H4; inversion H5.
+(* Case OrT *)
+apply sym_orthos.
+apply orthos_or1.
+apply sym_orthos.
+apply IHOrtho; auto. inversion H0. auto.
+apply sym_orthos.
+apply orthos_or2.
+apply sym_orthos.
+apply IHOrtho; auto. inversion H0. auto.
+apply orthos_or1.
+apply IHOrtho; auto. inversion H. auto.
+apply orthos_or2.
+apply IHOrtho; auto. inversion H. auto.
 Defined.
